feat: reduceNat.WF

Lean4Lean/Verify/TypeChecker/Theorems.lean
@@ -135,7 +135,7 @@ structure VContext extends Context where
   venv_wf : VEnv.WF venv
   hasPrimitives : VEnv.HasPrimitives venv
   safePrimitives : env.find? n = some ci →
-    Environment.primitives.contains n → isAsSafeAs .safe ci
+    Environment.primitives.contains n → isAsSafeAs .safe ci ∧ ci.levelParams = []
   trenv : TrEnv safety env venv
   mlctx : MLCtx
   mlctx_wf : mlctx.WF venv lparams
@@ -290,6 +290,9 @@ theorem RecM.WF.throw {c : VContext} {s : VState} {Q} : (throw e : RecM α).WF c
 theorem RecM.WF.le {c : VContext} {s : VState} {Q R} {x : RecM α}
     (h1 : x.WF c s Q) (H : ∀ a s', s ≤ s' → Q a s' → R a s') :
     x.WF c s R := fun _ h => (h1 _ h).le H
+
+theorem RecM.WF.pureBind {c : VContext} {s : VState} {f : β → RecM α} {Q}
+    {x : β} (H : WF c s (f x) Q) : ((Pure.pure x : RecM β) >>= f).WF c s Q := H
 
 theorem get.WF {c : VContext} {s : VState} :
     M.WF c s get fun a s' => s.toState = a ∧ s = s' := by
@@ -1228,7 +1231,7 @@ theorem literal_typeName_is_primitive {l : Literal} :
 theorem infer_literal {c : VContext} (H : c.venv.contains l.typeName) :
     c.TrTyping (.lit l) l.type (.trLiteral l) (.const l.typeName []) := by
   refine
-    have := TrExprS.trLiteral c.venv_wf c.hasPrimitives H
+    have := TrExprS.trLiteral c.venv_wf c.hasPrimitives l H
     ⟨fun _ _ _ => .litType, this.1, ?_, this.2⟩
   rw [← Literal.mkConst_typeName]
   have ⟨_, h⟩ := this.2.isType c.venv_wf c.mlctx_wf.tr.wf
@@ -1270,7 +1273,7 @@ theorem inferType'.WF
   · extract_lets n G1; split
     · refine .getEnv <| (M.WF.liftExcept envGet.WF).lift.bind fun _ _ _ h => ?_
       have ⟨_, h, _⟩ := c.trenv.find? h <|
-        isAsSafeAs_of_safe <| c.safePrimitives h literal_typeName_is_primitive
+        isAsSafeAs_of_safe (c.safePrimitives h literal_typeName_is_primitive).1
       simp [n, G1]; exact hF (infer_literal ⟨_, h⟩)
     · rename_i h; have ⟨_, h⟩ := hinf (by simpa using h)
       have := h.lit_has_type c.venv_wf c.hasPrimitives
@@ -1454,3 +1457,220 @@ theorem whnfCore'.WF {c : VContext} {s : VState} (he : c.TrExprS e e') :
       refine (whnfCore.WF h2).bind fun _ _ _ ⟨h3, h4⟩ => ?_
       exact hsave (h1.trans h3) (h4.defeq c.venv_wf c.mlctx_wf.tr.wf eq)
     · exact hsave .rfl (he.trExpr c.venv_wf c.mlctx_wf.tr.wf)
+
+theorem isDelta.WF (H : isDelta env e = some ci) :
+    ∃ n, env.find? n = some ci ∧ ci.hasValue ∧ ∃ ls, e.getAppFn = .const n ls := by
+  simp [isDelta] at H
+  split at H <;> [split at H; cases H] <;> [split at H; cases H] <;> cases H
+  exact ⟨_, ‹_›, ‹_›, _, ‹_›⟩
+
+theorem reduceNative.WF :
+    (reduceNative env e).WF fun oe => ∀ e₁, oe = some e₁ → False := by
+  unfold reduceNative; split <;> [skip; exact .pure nofun]
+  split <;> [exact .throw; skip]; split <;> [exact .throw; exact .pure nofun]
+
+theorem rawNatLitExt?.WF {c : VContext} (H : rawNatLitExt? e = some n) (he : c.TrExprS e e') :
+    c.venv.contains ``Nat ∧ e' = .natLit n := by
+  have : c.TrExprS (.lit (.natVal n)) e' := by
+    unfold rawNatLitExt? at H; split at H <;> rename_i h
+    · cases H; exact .lit (he.eqv h)
+    · unfold Expr.rawNatLit? at H; split at H <;> cases H; exact he
+  have hn := this.lit_has_type c.venv_wf c.hasPrimitives
+  exact ⟨hn, this.unique (by trivial) (TrExprS.natLit c.hasPrimitives hn n).1⟩
+
+def reduceBinNatOpG (guard : Nat → Nat → Prop) [DecidableRel guard]
+    (f : Nat → Nat → Nat) (a b : Expr) : RecM (Option Expr) := do
+  let some v1 := rawNatLitExt? (← whnf a) | return none
+  let some v2 := rawNatLitExt? (← whnf b) | return none
+  if guard v1 v2 then return none
+  return some <| .lit <| .natVal <| f v1 v2
+
+theorem reduceBinNatOpG.WF {guard} [DecidableRel guard] {c : VContext}
+    (he : c.TrExprS (.app (.app (.const fc ls) a) b) e')
+    (hprim : Environment.primitives.contains fc)
+    (heval : c.venv.contains fc → ∀ m n, c.IsDefEqU
+      (.app (.app (.const fc []) (.natLit m)) (.natLit n)) (.natLit (f m n))) :
+    RecM.WF c s (reduceBinNatOpG guard f a b) fun oe _ => ∀ e₁, oe = some e₁ →
+      c.FVarsBelow (.app (.app (.const fc ls) a) b) e₁ ∧ c.TrExpr e₁ e' := by
+  let .app hb1 hb2 hf hb := he
+  let .app ha1 ha2 hf ha := hf
+  let .const h1 h2 h3 := hf
+  unfold reduceBinNatOpG
+  refine (whnf.WF ha).bind fun a₁ _ _ ⟨a1, _, a2, a3⟩ => ?_
+  split <;> [rename_i h; exact .pure nofun]
+  obtain ⟨hn, rfl⟩ := rawNatLitExt?.WF h a2
+  refine (whnf.WF hb).bind fun b₁ _ _ ⟨b1, _, b2, b3⟩ => ?_
+  split <;> [rename_i h; exact .pure nofun]
+  cases (rawNatLitExt?.WF h b2).2
+  split <;> [exact .pure nofun; rename_i h]
+  refine .pure ?_; rintro _ ⟨⟩; refine ⟨fun _ _ _ => trivial, ?_⟩
+  have ⟨ci, c1⟩ := c.trenv.find?_iff.2 ⟨_, h1⟩
+  have ⟨c2, c3⟩ := c.safePrimitives c1 hprim
+  have ⟨d1, d2, d3⟩ := c.trenv.find?_uniq c1 h1
+  simp [c3] at d2; simp [← d2] at h3; simp [h3] at h2; subst h2
+  refine ⟨_, (TrExprS.natLit c.hasPrimitives hn _).1, ?_⟩
+  refine (heval ⟨_, h1⟩ ..).symm.trans c.venv_wf c.mlctx_wf.tr.wf ?_
+  have a3 := a3.of_r c.venv_wf c.mlctx_wf.tr.wf ha2
+  have b3 := b3.of_r c.venv_wf c.mlctx_wf.tr.wf hb2
+  have := ha1.appDF a3 |>.toU.of_r c.venv_wf c.mlctx_wf.tr.wf hb1
+  exact ⟨_, .appDF this b3⟩
+
+theorem reduceBinNatPred.WF {c : VContext}
+    (he : c.TrExprS (.app (.app (.const fc ls) a) b) e')
+    (hprim : Environment.primitives.contains fc)
+    (heval : c.venv.contains fc → ∀ m n, c.IsDefEqU
+      (.app (.app (.const fc []) (.natLit m)) (.natLit n)) (.boolLit (f m n))) :
+    RecM.WF c s (reduceBinNatPred f a b) fun oe _ => ∀ e₁, oe = some e₁ →
+      c.FVarsBelow (.app (.app (.const fc ls) a) b) e₁ ∧ c.TrExpr e₁ e' := by
+  let .app hb1 hb2 hf hb := he
+  let .app ha1 ha2 hf ha := hf
+  let .const h1 h2 h3 := hf
+  unfold reduceBinNatPred
+  refine (whnf.WF ha).bind fun a₁ _ _ ⟨a1, _, a2, a3⟩ => ?_
+  split <;> [rename_i h; exact .pure nofun]; cases (rawNatLitExt?.WF h a2).2
+  refine (whnf.WF hb).bind fun b₁ _ _ ⟨b1, _, b2, b3⟩ => ?_
+  split <;> [rename_i h; exact .pure nofun]; cases (rawNatLitExt?.WF h b2).2
+  refine .pure ?_; rintro _ ⟨⟩; refine ⟨fun _ _ _ => .boolLit, ?_⟩
+  have ⟨ci, c1⟩ := c.trenv.find?_iff.2 ⟨_, h1⟩
+  have ⟨c2, c3⟩ := c.safePrimitives c1 hprim
+  have ⟨d1, d2, d3⟩ := c.trenv.find?_uniq c1 h1
+  simp [c3] at d2; simp [← d2] at h3; simp [h3] at h2; subst h2
+  refine
+    have H := heval ⟨_, h1⟩ _ _
+    ⟨_, (TrExprS.boolLit c.hasPrimitives ?_ _).1, H.symm.trans c.venv_wf c.mlctx_wf.tr.wf ?_⟩
+  · let ⟨_, H⟩ := H
+    exact VExpr.WF.boolLit_has_type c.venv_wf c.hasPrimitives c.mlctx_wf.tr.wf ⟨_, H.hasType.2⟩
+  have a3 := a3.of_r c.venv_wf c.mlctx_wf.tr.wf ha2
+  have b3 := b3.of_r c.venv_wf c.mlctx_wf.tr.wf hb2
+  have := ha1.appDF a3 |>.toU.of_r c.venv_wf c.mlctx_wf.tr.wf hb1
+  exact  ⟨_, .appDF this b3⟩
+
+theorem natSucc_wf {c : VContext} (hf : c.venv.contains ``Nat.succ) (n) :
+    c.IsDefEqU (.app (.const ``Nat.succ []) (.natLit n)) (.natLit (Nat.succ n)) := sorry
+
+theorem natAdd_wf {c : VContext} (hf : c.venv.contains ``Nat.add) (m n) :
+    c.IsDefEqU (.app (.app (.const ``Nat.add []) (.natLit m)) (.natLit n))
+      (.natLit (Nat.add m n)) := sorry
+
+theorem natSub_wf {c : VContext} (hf : c.venv.contains ``Nat.sub) (m n) :
+    c.IsDefEqU (.app (.app (.const ``Nat.sub []) (.natLit m)) (.natLit n))
+      (.natLit (Nat.sub m n)) := sorry
+
+theorem natMul_wf {c : VContext} (hf : c.venv.contains ``Nat.mul) (m n) :
+    c.IsDefEqU (.app (.app (.const ``Nat.mul []) (.natLit m)) (.natLit n))
+      (.natLit (Nat.mul m n)) := sorry
+
+theorem natPow_wf {c : VContext} (hf : c.venv.contains ``Nat.pow) (m n) :
+    c.IsDefEqU (.app (.app (.const ``Nat.pow []) (.natLit m)) (.natLit n))
+      (.natLit (Nat.pow m n)) := sorry
+
+theorem natGcd_wf {c : VContext} (hf : c.venv.contains ``Nat.gcd) (m n) :
+    c.IsDefEqU (.app (.app (.const ``Nat.gcd []) (.natLit m)) (.natLit n))
+      (.natLit (Nat.gcd m n)) := sorry
+
+theorem natMod_wf {c : VContext} (hf : c.venv.contains ``Nat.mod) (m n) :
+    c.IsDefEqU (.app (.app (.const ``Nat.mod []) (.natLit m)) (.natLit n))
+      (.natLit (Nat.mod m n)) := sorry
+
+theorem natDiv_wf {c : VContext} (hf : c.venv.contains ``Nat.div) (m n) :
+    c.IsDefEqU (.app (.app (.const ``Nat.div []) (.natLit m)) (.natLit n))
+      (.natLit (Nat.div m n)) := sorry
+
+theorem natBEq_wf {c : VContext} (hf : c.venv.contains ``Nat.beq) (m n) :
+    c.IsDefEqU (.app (.app (.const ``Nat.beq []) (.natLit m)) (.natLit n))
+      (.boolLit (Nat.beq m n)) := sorry
+
+theorem natBLE_wf {c : VContext} (hf : c.venv.contains ``Nat.ble) (m n) :
+    c.IsDefEqU (.app (.app (.const ``Nat.ble []) (.natLit m)) (.natLit n))
+      (.boolLit (Nat.ble m n)) := sorry
+
+theorem natLAnd_wf {c : VContext} (hf : c.venv.contains ``Nat.land) (m n) :
+    c.IsDefEqU (.app (.app (.const ``Nat.land []) (.natLit m)) (.natLit n))
+      (.natLit (Nat.land m n)) := sorry
+
+theorem natLOr_wf {c : VContext} (hf : c.venv.contains ``Nat.lor) (m n) :
+    c.IsDefEqU (.app (.app (.const ``Nat.lor []) (.natLit m)) (.natLit n))
+      (.natLit (Nat.lor m n)) := sorry
+
+theorem natXor_wf {c : VContext} (hf : c.venv.contains ``Nat.xor) (m n) :
+    c.IsDefEqU (.app (.app (.const ``Nat.xor []) (.natLit m)) (.natLit n))
+      (.natLit (Nat.xor m n)) := sorry
+
+theorem natShiftLeft_wf {c : VContext} (hf : c.venv.contains ``Nat.shiftLeft) (m n) :
+    c.IsDefEqU (.app (.app (.const ``Nat.shiftLeft []) (.natLit m)) (.natLit n))
+      (.natLit (Nat.shiftLeft m n)) := sorry
+
+theorem natShiftRight_wf {c : VContext} (hf : c.venv.contains ``Nat.shiftRight) (m n) :
+    c.IsDefEqU (.app (.app (.const ``Nat.shiftRight []) (.natLit m)) (.natLit n))
+      (.natLit (Nat.shiftRight m n)) := sorry
+
+theorem reduceNat.WF {c : VContext} (he : c.TrExprS e e') :
+    RecM.WF c s (reduceNat e) fun oe _ => ∀ e₁, oe = some e₁ →
+      c.FVarsBelow e e₁ ∧ c.TrExpr e₁ e' := by
+  generalize hP : (fun oe => _) = P
+  refine let prims := _; have hprims : Environment.primitives = .ofList prims := rfl; ?_
+  replace hprims {a} : Environment.primitives.contains a ↔ a ∈ prims := by
+    simp [hprims, NameSet.contains, NameSet.ofList]
+  unfold reduceNat
+  extract_lets nargs F1 fn F2
+  split <;> [exact hP ▸ .pure nofun; refine .pureBind ?_]
+  unfold F2; split <;> (split <;> [skip; exact hP ▸ .pure nofun])
+  · rename_i _ h1 h2
+    simp [nargs, Expr.getAppNumArgs_eq] at h1; subst fn
+    let .app f a := e; simp [Expr.appFn!, Expr.eqv_const] at h2 ⊢; subst h2
+    let .app ha1 ha2 hf ha := he
+    let .const h1 h2 h3 := hf
+    refine (whnf.WF ha).bind fun a₁ _ _ ⟨a1, _, a2, a3⟩ => ?_
+    split <;> [rename_i h; exact hP ▸ .pure nofun]
+    obtain ⟨hn, rfl⟩ := rawNatLitExt?.WF h a2
+    refine hP ▸ .pure ?_; rintro _ ⟨⟩; refine ⟨fun _ _ _ => trivial, ?_⟩
+    have ⟨ci, c1⟩ := c.trenv.find?_iff.2 ⟨_, h1⟩
+    have ⟨c2, c3⟩ := c.safePrimitives c1 <| hprims.2 (by simp [prims])
+    have ⟨d1, d2, d3⟩ := c.trenv.find?_uniq c1 h1; cases h2
+    refine ⟨_, (TrExprS.natLit c.hasPrimitives hn _).1, ?_⟩
+    refine (natSucc_wf ⟨_, h1⟩ ..).symm.trans c.venv_wf c.mlctx_wf.tr.wf ?_
+    exact ⟨_, ha1.appDF <| a3.of_r c.venv_wf c.mlctx_wf.tr.wf ha2⟩
+  · split <;> [rename_i f ls a b _ _ h2; exact hP ▸ .pure nofun]
+    dsimp
+    have hfun {g fc G}
+        (hprim : fc ∈ prims)
+        (heval : c.venv.contains fc → ∀ m n, c.IsDefEqU
+          (.app (.app (.const fc []) (.natLit m)) (.natLit n)) (.natLit (g m n)))
+        (hG : RecM.WF c s G P) :
+        RecM.WF c s (if f == fc then return (← reduceBinNatOp g a b) else G) P := by
+      split <;> [rename_i h; exact hG]
+      simp at h ⊢; subst h
+      refine hP ▸ reduceBinNatOpG.WF (guard := fun _ _ => False) he (hprims.2 hprim) heval
+    have hpow {fc G}
+        (hprim : fc ∈ prims)
+        (heval : c.venv.contains fc → ∀ m n, c.IsDefEqU
+          (.app (.app (.const fc []) (.natLit m)) (.natLit n)) (.natLit (Nat.pow m n)))
+        (hG : RecM.WF c s G P) :
+        RecM.WF c s (if f == fc then return (← reducePow a b) else G) P := by
+      split <;> [rename_i h; exact hG]
+      simp at h ⊢; subst h
+      refine hP ▸ reduceBinNatOpG.WF he (hprims.2 hprim) heval
+    have hpred {g fc G}
+        (hprim : fc ∈ prims)
+        (heval : c.venv.contains fc → ∀ m n, c.IsDefEqU
+          (.app (.app (.const fc []) (.natLit m)) (.natLit n)) (.boolLit (g m n)))
+        (hG : RecM.WF c s G P) :
+        RecM.WF c s (if f == fc then return (← reduceBinNatPred g a b) else G) P := by
+      split <;> [rename_i h; exact hG]
+      simp at h ⊢; subst h
+      refine hP ▸ reduceBinNatPred.WF he (hprims.2 hprim) heval
+    refine hfun (by simp [prims]) natAdd_wf ?_
+    refine hfun (by simp [prims]) natSub_wf ?_
+    refine hfun (by simp [prims]) natMul_wf ?_
+    refine hpow (by simp [prims]) natPow_wf ?_
+    refine hfun (by simp [prims]) natGcd_wf ?_
+    refine hfun (by simp [prims]) natMod_wf ?_
+    refine hfun (by simp [prims]) natDiv_wf ?_
+    refine hpred (by simp [prims]) natBEq_wf ?_
+    refine hpred (by simp [prims]) natBLE_wf ?_
+    refine hfun (by simp [prims]) natLAnd_wf ?_
+    refine hfun (by simp [prims]) natLOr_wf ?_
+    refine hfun (by simp [prims]) natXor_wf ?_
+    refine hfun (by simp [prims]) natShiftLeft_wf ?_
+    refine hfun (by simp [prims]) natShiftRight_wf ?_
+    exact hP ▸ .pure nofun
